---
title: 第3节 高阶导数
weight: 3
---
## 一、基础题

### 1 求下列函数的二阶导数

(1) $y = x\sin x$

解答：
$$y' = \sin x + x\cos x$$
$$y'' = \cos x + \cos x - x\sin x = 2\cos x - x\sin x$$

(2) $y = e^{-x}\sin x$

解答：
$$y' = e^{-x}(\cos x - \sin x)$$
$$y'' = e^{-x}(-\sin x - \cos x) - e^{-x}(\cos x - \sin x)$$
$$= e^{-x}(-2\cos x)$$

(3) $y=\sqrt{a^{2}-x^{2}}$

解答：
$$y'=\frac{-x}{\sqrt{a^{2}-x^{2}}}$$
$$y''=\frac{-\sqrt{a^{2}-x^{2}}-(-x)\frac{-x}{\sqrt{a^{2}-x^{2}}}}{a^{2}-x^{2}}$$
$$=\frac{-a^{2}}{(a^{2}-x^{2})^{3/2}}$$

(4) $y=\ln(1+5x^{2})$

解答：
$$y'=\frac{10x}{1+5x^{2}}$$
$$y''=\frac{10(1+5x^{2})-10x\cdot 10x}{(1+5x^{2})^{2}}$$
$$=\frac{10-50x^{2}}{(1+5x^{2})^{2}}$$

(5) $y=\cos x+\tan x$

解答：
$$y'=-\sin x+\sec^{2}x$$
$$y''=-\cos x+2\sec^{2}x\tan x$$

(6) $y=\frac{1}{x^{3}+1}$

解答：
$$y'= -\frac{3x^{2}}{(x^{3}+1)^{2}}$$
$$y''= -\frac{6x(x^{3}+1)^{2}-3x^{2}\cdot 2(x^{3}+1)\cdot 3x^{2}}{(x^{3}+1)^{4}}$$
$$= \frac{-6x(x^{3}+1)+18x^{4}}{(x^{3}+1)^{3}}$$

### 2 设 $f''(x)$ 存在，求下列函数的二阶导数 $\frac{d^{2}y}{dx^{2}}$

(1) $y=f^{2}(x)$

解答：
$$y'=2f(x)f'(x)$$
$$y''=2[f'(x)]^{2}+2f(x)f''(x)$$

(2) $y=f(\ln x)$

解答：
$$y'=f'(\ln x)\frac1x$$
$$y''=f''(\ln x)\frac1{x^{2}} - f'(\ln x)\frac1{x^{2}}$$

(3) $y=f(x^{n})$

解答：
$$y'=f'(x^{n})nx^{n-1}$$
$$y''=f''(x^{n})(nx^{n-1})^{2}+f'(x^{n})n(n-1)x^{n-2}$$

(4) $y=f[l f(x)]$

解答：
设 $u=lf(x)$，则：
$$y'=f'(u)\cdot l f'(x)$$
$$y''=f''(u)(l f'(x))^{2} + f'(u)\cdot l f''(x)$$

## 二、提高题

### 3 求下列函数的 $n$ 阶导数

(1) $y=\frac{1-x}{1+x}$

解答：
写成：
$$y= -1+\frac{2}{1+x}$$
$$y^{(n)} = 2(-1)^{n}n!(1+x)^{-n-1}$$

(2) $y=\frac{x^{3}}{1-x}\ (n\ge3)$

解答：
分解：
$$\frac{x^{3}}{1-x}= -x^{2}-x-1-\frac{1}{1-x}$$
前三项的三阶以上导数为 0，因此：
$$y^{(n)} = -(-1)^{n}n!(1-x)^{-n-1}$$

(3) $y=\frac{1}{x^{2}-3x+2}$

解答：
因式分解：
$$y=\frac{1}{(x-1)(x-2)}=\frac{-1}{x-1}+\frac{1}{x-2}$$
$$y^{(n)} = -(-1)^{n}n!(x-1)^{-n-1} + (-1)^{n}n!(x-2)^{-n-1}$$

(4) $y=\cos^{2}x$

解答：
$$y=\frac{1+\cos 2x}{2}$$
$$y^{(n)}=\frac{d^{n}}{dx^{n}}\left(\frac12+\frac12\cos 2x\right)$$
$$=\frac12 (2^{n})\cos\left(2x+\frac{n\pi}{2}\right)$$

(5) $y=\sin^{6}x+\cos^{6}x$

解答：
利用恒等式：
$$\sin^{6}x+\cos^{6}x = 1-\frac34\sin^{2}2x$$
$$y=1-\frac38+\frac38\cos4x$$
$$y^{(n)}=\frac38\cdot 4^{n}\cos\left(4x+\frac{n\pi}{2}\right)$$

(6) $y=x\ln x\ (n\ge2)$

解答：
$$y'=1+\ln x$$
$$y''=\frac1x$$
$$y^{(n)} = (-1)^{n-2}(n-2)! x^{-n+1}$$

(7) $y=xe^{x}$

解答：

$$y^{(n)} = x e^{x} + n e^{x}$$

### 4 设 $y=f(x)$，且 $\frac{dx}{dy}=\frac1{y'}$，证明

(1) $\frac{d^{2}x}{dy^{2}} = -\frac{y''}{(y')^{3}}$

解答：

$$\frac{dx}{dy}=\frac1{y'}$$

对 $y$ 再求导：
$$\frac{d^{2}x}{dy^{2}}=\frac{d}{dx}\left(\frac1{y'}\right)\cdot \frac{dx}{dy}$$
$$= -\frac{y''}{(y')^{2}}\cdot \frac1{y'}=-\frac{y''}{(y')^{3}}$$

(2) $\frac{d^{3}x}{dy^{3}} = -\frac{3(y'')^{2}-y'y'''}{(y')^{5}}$

解答：

从(1)继续：
$$\frac{d^{3}x}{dy^{3}}=\frac{d}{dx}\left(-\frac{y''}{(y')^{3}}\right)\cdot \frac{dx}{dy}$$

计算导数：
$$\frac{d}{dx}\left(-\frac{y''}{(y')^{3}}\right)=
-\frac{y'''(y')^{3}-3y''(y')^{2}y''}{(y')^{6}}$$
$$= -\frac{y'y''' - 3(y'')^{2}}{(y')^{4}}$$

乘上 $\frac1{y'}$：
$$\frac{d^{3}x}{dy^{3}}=
-\frac{y'y''' - 3(y'')^{2}}{(y')^{5}}$$
$$= -\frac{3(y'')^{2}-y'y'''}{(y')^{5}}$$
